Imp/interactions/int_ite_err.v
@@ -32,9 +32,27 @@ Section int_exp_ite.
     Variable preservation : forall c e c' e', lc' 0 e -> step c e c' e' -> lc' 0 e'.
 
     Inductive step_int_ite_err : Ctx -> exp -> Ctx -> exp -> Prop := 
+        | step_bad_cnd t f c e c' e': 
+            step c e c' (err_ _ e') -> 
+            step_int_ite_err c (ite_ _ e t f) c' (err_ _ e')
+        | step_bad_beta e t f c: 
+            value e  -> 
+            ~ tag_of e (tag_bool_ _) -> 
+            step_int_ite_err c (ite_ _ e t f) c (err_ _ e)
         . 
 
     Definition preservation_ite_err : forall c e c' e', lc' 0 e -> step_int_ite_err c e c' e' -> lc' 0 e'.
     Proof. 
-    Admitted.
+        intros c e c' e' lc_e.
+        induction 1. 
+        - apply retract_lc_err. constructor. apply preservation in H.
+            + apply retract_lc_rev_err in H. inversion H. 
+              apply retract_inj in H0. inversion H0. subst.
+              easy.
+            + apply retract_lc_rev_ite in lc_e. inversion lc_e. 
+              apply retract_inj in H0. inversion H0. { subst. easy. }
+              all: subst; apply retract_inj in H2; inversion H2.
+        - apply retract_lc_err. constructor. 
+          apply value_lc. easy. 
+    Defined.
 End int_exp_ite.
